Upd Point Add

code/ecdsap256/Hacl.Impl.P256.PointAdd.fst
@@ -19,7 +19,6 @@ open Hacl.Impl.P256.MontgomeryMultiplication
 open Spec.P256
 open Hacl.Impl.P256.Math 
 
-
 open FStar.Tactics 
 open FStar.Tactics.Canon
 
@@ -28,19 +27,19 @@ open FStar.Math.Lemmas
 friend Hacl.Spec.P256.MontgomeryMultiplication
 open FStar.Mul
 
-#reset-options "--z3rlimit 300" 
+
+#set-options "--z3rlimit 300" 
 
 noextract       
 val lemma_pointAddToSpecification: 
   #c: curve -> 
-  pxD: nat {pxD < getPrime c} -> pyD: nat{pyD < getPrime c} -> pzD: nat {pzD < getPrime c} -> 
+  pxD: nat {pxD < getPrime c} -> pyD: nat {pyD < getPrime c} -> pzD: nat {pzD < getPrime c} -> 
   qxD: nat {qxD < getPrime c} -> qyD: nat {qyD < getPrime c} -> qzD: nat {qzD < getPrime c} -> 
   x3: nat -> y3: nat -> z3: nat -> 
   u1: nat -> u2: nat -> s1: nat -> s2: nat -> 
   h: nat -> r: nat -> 
   Lemma
     (requires (    
-
       let prime = getPrime c in 
       
       let x3D, y3D, z3D = fromDomain_ #c x3, fromDomain_ #c y3, fromDomain_ #c z3 in 
@@ -50,24 +49,24 @@ val lemma_pointAddToSpecification:
       let rD = fromDomain_ #c r in    
       let hD = fromDomain_ #c h in 
      
-      u1 == toDomain_ #c (qzD * qzD * pxD % prime256) /\
-      u2 == toDomain_ #c (pzD * pzD * qxD % prime256) /\
-      s1 == toDomain_ #c (qzD * qzD * qzD * pyD % prime256) /\
-      s2 == toDomain_ #c (pzD * pzD * pzD * qyD % prime256) /\
+      u1 == toDomain_ #c (qzD * qzD * pxD % prime) /\
+      u2 == toDomain_ #c (pzD * pzD * qxD % prime) /\
+      s1 == toDomain_ #c (qzD * qzD * qzD * pyD % prime) /\
+      s2 == toDomain_ #c (pzD * pzD * pzD * qyD % prime) /\
       
-      h == toDomain_ #c ((u2D - u1D) % prime256) /\
-      r == toDomain_ #c ((s2D - s1D) % prime256) /\
+      h == toDomain_ #c ((u2D - u1D) % prime) /\
+      r == toDomain_ #c ((s2D - s1D) % prime) /\
       (
-  if qzD = 0 then 
-    fromDomain_ #c x3 == pxD /\ fromDomain_ #c y3 == pyD /\ fromDomain_ #c z3 == pzD
-  else if pzD = 0 then 
-      fromDomain_ #c x3  == qxD /\  fromDomain_ #c y3 == qyD /\ fromDomain_ #c z3 == qzD 
-  else
-      x3 == toDomain_ #c ((rD * rD - hD * hD * hD - 2 * hD * hD * u1D) % prime) /\
-      y3 == toDomain_ #c (((hD * hD * u1D - x3D) * rD - s1D * hD*hD*hD) % prime) /\
-      z3 == toDomain_ #c ((pzD * qzD * hD) % prime)
-  )
+      if qzD = 0 then 
+	fromDomain_ #c x3 == pxD /\ fromDomain_ #c y3 == pyD /\ fromDomain_ #c z3 == pzD
+      else if pzD = 0 then 
+	fromDomain_ #c x3  == qxD /\ fromDomain_ #c y3 == qyD /\ fromDomain_ #c z3 == qzD 
+      else
+	x3 == toDomain_ #c ((rD * rD - hD * hD * hD - 2 * hD * hD * u1D) % prime) /\
+	y3 == toDomain_ #c (((hD * hD * u1D - x3D) * rD - s1D * hD*hD*hD) % prime) /\
+	z3 == toDomain_ #c ((pzD * qzD * hD) % prime)
       )
+    )
   )
   (ensures 
   (    
@@ -79,9 +78,12 @@ val lemma_pointAddToSpecification:
   )
 )
 
+
 let lemma_pointAddToSpecification #c x1D y1D z1D x2D y2D z2D x3 y3 z3  u1 u2 s1 s2 h r = 
   let open FStar.Tactics in 
   let open FStar.Tactics.Canon in 
+
+  let prime = getPrime c in 
    
   let u1D = fromDomain_ #c u1 in 
   let u2D = fromDomain_ #c u2 in 
@@ -100,66 +102,63 @@ let lemma_pointAddToSpecification #c x1D y1D z1D x2D y2D z2D x3 y3 z3  u1 u2 s1 
 
      let prime = getPrime c in 
 
-      u1 == toDomain_ #c (z2D * z2D * pxD % prime256) /\
-      u2 == toDomain_ #c (pzD * pzD * qxD % prime256) /\
-      s1 == toDomain_ #c (qzD * qzD * qzD * pyD % prime256) /\
-      s2 == toDomain_ #c (pzD * pzD * pzD * qyD % prime256) /\
+      u1 == toDomain_ #c (z2D * z2D * pxD % prime) /\
+      u2 == toDomain_ #c (pzD * pzD * qxD % prime) /\
+      s1 == toDomain_ #c (qzD * qzD * qzD * pyD % prime) /\
+      s2 == toDomain_ #c (pzD * pzD * pzD * qyD % prime) /\
       
-      h == toDomain_ #c ((u2D - u1D) % prime256) /\
-      r == toDomain_ #c ((s2D - s1D) % prime256) /\
+      h == toDomain_ #c ((u2D - u1D) % prime) /\
+      r == toDomain_ #c ((s2D - s1D) % prime) /\
       (
-  if qzD = 0 then 
-     x3D == pxD /\ y3D == pyD /\  z3D == pzD
-  else if pzD = 0 then 
-       x3D == qxD /\ y3D == qyD /\ z3D == qzD 
-  else
-      x3 == toDomain_ #c ((rD * rD - hD * hD * hD - 2 * hD * hD * u1D) % prime) /\
-      y3 == toDomain_ #c (((hD * hD * u1D - x3D) * rD - s1D * hD * hD * hD) % prime) /\
-      z3 == toDomain_ #c ((pzD * qzD * hD) % prime)
-  )
-      );
+      if qzD = 0 then 
+	x3D == pxD /\ y3D == pyD /\  z3D == pzD
+      else if pzD = 0 then 
+	x3D == qxD /\ y3D == qyD /\ z3D == qzD 
+      else
+	x3 == toDomain_ #c ((rD * rD - hD * hD * hD - 2 * hD * hD * u1D) % prime) /\
+	y3 == toDomain_ #c (((hD * hD * u1D - x3D) * rD - s1D * hD * hD * hD) % prime) /\
+	z3 == toDomain_ #c ((pzD * qzD * hD) % prime)));
 
-    let (xN, yN, zN) = _point_add #c (x1D, y1D, z1D) (x2D, y2D, z2D) in 
+  let (xN, yN, zN) = _point_add #c (x1D, y1D, z1D) (x2D, y2D, z2D) in 
 
+  assert_by_tactic (z2D * z2D * pxD = pxD * (z2D * z2D)) canon; 
+  assert_by_tactic (z1D * z1D * x2D == x2D * (z1D * z1D)) canon;
 
-    assert_by_tactic (z2D * z2D * pxD = pxD * (z2D * z2D)) canon; 
-    assert_by_tactic (z1D * z1D * x2D == x2D * (z1D * z1D)) canon;
-
-    assert_by_tactic (z2D * z2D * z2D * y1D = y1D * z2D * (z2D * z2D)) canon;
-    assert_by_tactic (z1D * z1D * z1D * y2D = y2D * z1D * (z1D * z1D)) canon;
+  assert_by_tactic (z2D * z2D * z2D * y1D = y1D * z2D * (z2D * z2D)) canon;
+  assert_by_tactic (z1D * z1D * z1D * y2D = y2D * z1D * (z1D * z1D)) canon;
 
   let z2z2 = z2D * z2D in
   let z1z1 = z1D * z1D in
 
-  let u1 = x1D * z2z2 % prime256 in
-  let u2 = x2D * z1z1 % prime256 in
+  let u1 = x1D * z2z2 % prime in
+  let u2 = x2D * z1z1 % prime in
 
-  let s1 = y1D * z2D * z2z2 % prime256 in
-  let s2 = y2D * z1D * z1z1 % prime256 in
+  let s1 = y1D * z2D * z2z2 % prime in
+  let s2 = y2D * z1D * z1z1 % prime in
 
   assert(u1 == u1D);
   assert(u2 == u2D);
   assert(s1 == s1D);
   assert(s2 == s2D);
 
-  let h = (u2 - u1) % prime256 in
+  let h = (u2 - u1) % prime in
   assert(h == hD);
   
-  let r = (s2 - s1) % prime256 in
+  let r = (s2 - s1) % prime in
   assert(r == rD);
 
   let rr = r * r in
   let hh = h * h in
   let hhh = h * h * h in
 
-  let x3_ = (r * r - h * h * h - 2 * u1 * hh) % prime256 in 
+  let x3_ = (r * r - h * h * h - 2 * u1 * hh) % prime in 
     assert_by_tactic (2 * u1 * (h * h) == 2 * h * h * u1) canon;
 
-  let y3_ = (r * (u1 * (h * h) - x3_) - s1 * (h * h * h)) % prime256 in
+  let y3_ = (r * (u1 * (h * h) - x3_) - s1 * (h * h * h)) % prime in
     assert_by_tactic ((h * h * u1 - x3_) == (u1 * (h * h) - x3_)) canon;
     assert_by_tactic ((r * (h * h * u1 - x3_) - s1 * (h * h * h)) = ((h * h * u1 - x3_) * r - s1 * h * h * h)) canon; 
 
-  let z3_ = (h * z1D * z2D) % prime256 in 
+  let z3_ = (h * z1D * z2D) % prime in 
     
     assert_by_tactic (z1D * z2D * hD = hD * z1D * z2D) canon;
 
@@ -172,410 +171,468 @@ let lemma_pointAddToSpecification #c x1D y1D z1D x2D y2D z2D x3 y3 z3  u1 u2 s1 
       assert(xN == x3_ /\ yN == y3_ /\ zN == z3_)
       
 
-val lemma_point_add_0: a: int -> b: int -> c: int -> Lemma 
-  ((a - b - 2 * (c % prime256)) % prime256 == (a - b - 2 * c) % prime256)
+val lemma_point_add_0: #cu: curve -> a: int -> b: int -> c: int -> Lemma 
+  (
+    let prime = getPrime cu in 
+    (a - b - 2 * (c % prime)) % prime == (a - b - 2 * c) % prime)
 
-let lemma_point_add_0 a b c = 
-  lemma_mod_sub_distr (a - b) (2 * (c % prime256)) prime256;
-  lemma_mod_mul_distr_r 2 c prime256;
-  lemma_mod_sub_distr (a - b) (2 * c) prime256
+let lemma_point_add_0 #cu a b c = 
+  let prime = getPrime cu in 
+  lemma_mod_sub_distr (a - b) (2 * (c % prime)) prime;
+  lemma_mod_mul_distr_r 2 c prime;
+  lemma_mod_sub_distr (a - b) (2 * c) prime
 
 
-val lemma_point_add_1: a: int -> b: int -> c: int -> d: int -> e: int -> Lemma
-  ((((a % prime256) - b) * c - d * (e % prime256)) % prime256 == ((a - b) * c - d * e) % prime256)
+val lemma_point_add_1: #cu: curve -> a: int -> b: int -> c: int -> d: int -> e: int -> Lemma
+  (
+    let prime = getPrime cu in 
+    (((a % prime) - b) * c - d * (e % prime)) % prime == ((a - b) * c - d * e) % prime)
 
-let lemma_point_add_1 a b c d e = 
-  lemma_mod_add_distr (- d * (e % prime256)) (((a % prime256) - b) * c) prime256;
-  lemma_mod_mul_distr_l ((a % prime256) - b) c prime256;
-  lemma_mod_add_distr (-b) a prime256;
-  lemma_mod_mul_distr_l (a - b) c prime256;
-  lemma_mod_add_distr (- d * (e % prime256)) ((a - b) * c) prime256;
-  
-  lemma_mod_sub_distr ((a - b) * c) (d * (e % prime256)) prime256;
-  lemma_mod_mul_distr_r d e prime256;
-  lemma_mod_sub_distr ((a - b) * c) (d * e) prime256
+let lemma_point_add_1 #cu a b c d e = 
+  let prime = getPrime cu in 
+  lemma_mod_add_distr (- d * (e % prime)) (((a % prime) - b) * c) prime;
+  lemma_mod_mul_distr_l ((a % prime) - b) c prime;
+  lemma_mod_add_distr (-b) a prime;
+  lemma_mod_mul_distr_l (a - b) c prime;
+  lemma_mod_add_distr (- d * (e % prime)) ((a - b) * c) prime;
+ 
+  lemma_mod_sub_distr ((a - b) * c) (d * (e % prime)) prime;
+  lemma_mod_mul_distr_r d e prime;
+  lemma_mod_sub_distr ((a - b) * c) (d * e) prime
 
 
 
 val copy_point_conditional: #c: curve ->  x3_out: felem c -> y3_out: felem c -> z3_out: felem c -> p: point c -> maskPoint: point c -> Stack unit
   (requires fun h -> live h x3_out /\ live h y3_out /\ live h z3_out /\ live h p /\ live h maskPoint /\ 
-    LowStar.Monotonic.Buffer.all_disjoint[loc x3_out; loc y3_out; loc z3_out; loc p; loc maskPoint] /\
+    LowStar.Monotonic.Buffer.all_disjoint [loc x3_out; loc y3_out; loc z3_out; loc p; loc maskPoint] /\
       (
 	let prime = getPrime c in 
-	as_nat c h x3_out < prime /\ as_nat c h y3_out < prime /\ as_nat c h z3_out < prime /\
-	as_nat c h (gsub p (size 0) (size 4)) < prime /\ 
-	as_nat c h (gsub p (size 4) (size 4)) < prime /\ 
-	as_nat c h (gsub p (size 8) (size 4)) < prime 
+	let len = getCoordinateLenU64 c in 
+	as_nat c h x3_out < prime /\ as_nat c h y3_out < prime /\ as_nat c h z3_out < prime  /\
+	as_nat c h (gsub p (size 0) len) < prime /\ 
+	as_nat c h (gsub p len len) < prime /\ 
+	as_nat c h (gsub p (size 2 *! len) len) < prime 
     )
   )
   (ensures fun h0 _ h1 -> modifies (loc x3_out |+| loc y3_out |+| loc z3_out) h0 h1 /\ 
     (
       let prime = getPrime c in 
-    as_nat c h1 x3_out < prime /\
-    as_nat c h1 y3_out < prime /\
-    as_nat c h1 z3_out < prime /\
-    (
-      let mask = as_nat c h0 (gsub maskPoint (size 8) (size 4)) in 
-      let x = gsub p (size 0) (size 4) in 
-      let y = gsub p (size 4) (size 4) in 
-      let z = gsub p (size 8) (size 4) in 
-
-      if mask = 0 then 
-	as_nat c h1 x3_out == as_nat c h0 x /\ 
-	as_nat c h1 y3_out == as_nat c h0 y /\ 
-	as_nat c h1 z3_out == as_nat c h0 z
-      else 
-	as_nat c h1 x3_out == as_nat c h0 x3_out /\ 
-	as_nat c h1 y3_out == as_nat c h0 y3_out /\ 
-	as_nat c h1 z3_out == as_nat c h0 z3_out
-    )
-   )
+      let len = getCoordinateLenU64 c in 
+      
+      as_nat c h1 x3_out < prime /\
+      as_nat c h1 y3_out < prime /\
+      as_nat c h1 z3_out < prime  /\
+      (
+	let coordinateMask = gsub maskPoint (size 2 *! len) len in 
+	let mask = as_nat c h0 coordinateMask in 
+	
+	let x, y, z = gsub p (size 0) len, gsub p len len, gsub p (size 2 *! len) len in
+	if mask = 0 then 
+	  as_nat c h1 x3_out == as_nat c h0 x /\ 
+	  as_nat c h1 y3_out == as_nat c h0 y /\ 
+	  as_nat c h1 z3_out == as_nat c h0 z
+	else 
+	  as_nat c h1 x3_out == as_nat c h0 x3_out /\ 
+	  as_nat c h1 y3_out == as_nat c h0 y3_out /\ 
+	  as_nat c h1 z3_out == as_nat c h0 z3_out
+	) 
+    ) 
 )
 
-let copy_point_conditional #c x3_out y3_out z3_out p maskPoint = 
-  let z = sub maskPoint (size 8) (size 4) in 
-  let mask = isZero_uint64_CT #c z in 
 
-  let p_x = sub p (size 0) (size 4) in 
-  let p_y = sub p (size 4) (size 4) in 
-  let p_z = sub p (size 8) (size 4) in 
+let copy_point_conditional #c x3_out y3_out z3_out p maskPoint = 
+  let len : FStar.UInt32.t = getCoordinateLenU64 c in 
+  
+  let z = sub maskPoint (size 2 *! len) len in 
+  let mask = isZero_uint64_CT #c z in 
+  
+  let p_x = sub p (size 0) len in 
+  let p_y = sub p len len in 
+  let p_z = sub p (size 2 *! len) len in 
 
   copy_conditional x3_out p_x mask;
   copy_conditional y3_out p_y mask;
   copy_conditional z3_out p_z mask
 
-    
+
 inline_for_extraction noextract 
 val move_from_jacobian_coordinates: #c: curve -> u1: felem c -> u2: felem c -> s1: felem c -> s2: felem c -> p: point c -> q: point c -> 
-  tempBuffer16: lbuffer uint64 (size 16) -> 
+  tempBuffer16: lbuffer uint64 (size 4 *! getCoordinateLenU64 c) -> 
   Stack unit (requires fun h -> live h u1 /\ live h u2 /\ live h s1 /\ live h s2 /\ live h p /\ live h q /\ live h tempBuffer16 /\
    LowStar.Monotonic.Buffer.all_disjoint [loc tempBuffer16; loc p; loc q; loc u1; loc u2; loc s1; loc s2] /\
      (
        let prime = getPrime c in 
-       as_nat c h (gsub p (size 8) (size 4)) < prime /\ 
-       as_nat c h (gsub p (size 0) (size 4)) < prime /\ 
-       as_nat c h (gsub p (size 4) (size 4)) < prime /\
-       as_nat c h (gsub q (size 8) (size 4)) < prime /\ 
-       as_nat c h (gsub q (size 0) (size 4)) < prime /\ 
-       as_nat c h (gsub q (size 4) (size 4)) < prime
+       let len = getCoordinateLenU64 c in 
+       
+       as_nat c h (gsub p (size 0) len) < prime /\ 
+       as_nat c h (gsub p len len) < prime /\ 
+       as_nat c h (gsub p (size 2 *! len) len) < prime /\
+       
+       as_nat c h (gsub q (size 0) len) < prime /\ 
+       as_nat c h (gsub q len len) < prime /\ 
+       as_nat c h (gsub q (size 2 *! len) len) < prime
      )
     )
   (ensures fun h0 _ h1 ->  
     modifies (loc u1 |+| loc u2 |+| loc s1 |+| loc s2 |+| loc tempBuffer16) h0 h1 /\
       (
 	let prime = getPrime c in 
+	let len = getCoordinateLenU64 c in 
+	
 	as_nat c h1 u1 < prime /\ as_nat c h1 u2 < prime /\ as_nat c h1 s1 < prime /\ as_nat c h1 s2 < prime  /\
 	(
-	let pX, pY, pZ = as_nat c h0 (gsub p (size 0) (size 4)), as_nat c h0 (gsub p (size 4) (size 4)), as_nat c h0 (gsub p (size 8) (size 4)) in 
-	let qX, qY, qZ = as_nat c h0 (gsub q (size 0) (size 4)), as_nat c h0 (gsub q (size 4) (size 4)), as_nat c h0 (gsub q (size 8) (size 4)) in 
+	let pX, pY, pZ = as_nat c h0 (gsub p (size 0) len), as_nat c h0 (gsub p len len), as_nat c h0 (gsub p (size 2 *! len) len) in 
+	let qX, qY, qZ = as_nat c h0 (gsub q (size 0) len), as_nat c h0 (gsub q len len), as_nat c h0 (gsub q (size 2 *! len) len) in 
       
-      let pxD, pyD, pzD = fromDomain_ #c pX, fromDomain_ #c pY, fromDomain_ #c pZ in 
-      let qxD, qyD, qzD = fromDomain_ #c qX, fromDomain_ #c qY, fromDomain_ #c qZ in 
+	let pxD, pyD, pzD = fromDomain_ #c pX, fromDomain_ #c pY, fromDomain_ #c pZ in 
+	let qxD, qyD, qzD = fromDomain_ #c qX, fromDomain_ #c qY, fromDomain_ #c qZ in 
 
-      as_nat c h1 u1 == toDomain_ #c (qzD * qzD * pxD % prime256) /\
-      as_nat c h1 u2 == toDomain_ #c (pzD * pzD * qxD % prime256) /\
-      as_nat c h1 s1 == toDomain_ #c (qzD * qzD * qzD * pyD % prime256) /\
-      as_nat c h1 s2 == toDomain_ #c (pzD * pzD * pzD * qyD % prime256)
-   )
-)
+	as_nat c h1 u1 == toDomain_ #c (qzD * qzD * pxD % prime) /\
+	as_nat c h1 u2 == toDomain_ #c (pzD * pzD * qxD % prime) /\
+	as_nat c h1 s1 == toDomain_ #c (qzD * qzD * qzD * pyD % prime) /\
+	as_nat c h1 s2 == toDomain_ #c (pzD * pzD * pzD * qyD % prime)
+    )
+  )
 )
 
 let move_from_jacobian_coordinates #c u1 u2 s1 s2 p q tempBuffer = 
-    let h0 = ST.get() in 
-   let pX = sub p (size 0) (size 4) in 
-   let pY = sub p (size 4) (size 4) in 
-   let pZ = sub p (size 8) (size 4) in 
+  let h0 = ST.get() in 
 
-   let qX = sub q (size 0) (size 4) in 
-   let qY = sub q (size 4) (size 4) in 
-   let qZ = sub q (size 8) (size 4) in 
+  let len = getCoordinateLenU64 c in 
+    
+  let pX = sub p (size 0) len in 
+  let pY = sub p len len in 
+  let pZ = sub p (size 2 *! len) len in 
 
-   let z2Square = sub tempBuffer (size 0) (size 4) in 
-   let z1Square = sub tempBuffer (size 4) (size 4) in 
-   let z2Cube = sub tempBuffer (size 8) (size 4) in 
-   let z1Cube = sub tempBuffer (size 12) (size 4) in  
+  let qX = sub q (size 0) len in 
+  let qY = sub q len len in 
+  let qZ = sub q (size 2 *! len) len in 
 
-   montgomery_square_buffer #c qZ z2Square;
-   montgomery_square_buffer #c pZ z1Square;
-   montgomery_multiplication_buffer #c z2Square qZ z2Cube;
+  let z2Square = sub tempBuffer (size 0) len in 
+  let z1Square = sub tempBuffer len len in 
+  let z2Cube = sub tempBuffer (size 2 *! len) len in 
+  let z1Cube = sub tempBuffer (size 3 *! len) len in  
+
+  montgomery_square_buffer #c qZ z2Square;
+  montgomery_square_buffer #c pZ z1Square;
+  montgomery_multiplication_buffer #c z2Square qZ z2Cube;
    
-   montgomery_multiplication_buffer #c z1Square pZ z1Cube;
-   montgomery_multiplication_buffer #c z2Square pX u1;
-   montgomery_multiplication_buffer #c  z1Square qX u2;
-   
-   montgomery_multiplication_buffer #c z2Cube pY s1;
-   montgomery_multiplication_buffer #c z1Cube qY s2;
-   () (*
+  montgomery_multiplication_buffer #c z1Square pZ z1Cube;
+  montgomery_multiplication_buffer #c z2Square pX u1;
+  montgomery_multiplication_buffer #c  z1Square qX u2;
+    
+  montgomery_multiplication_buffer #c z2Cube pY s1;
+  montgomery_multiplication_buffer #c z1Cube qY s2;
 
-     lemma_mod_mul_distr_l (fromDomain_ #c (as_nat c h0 qZ) * fromDomain_ #c (as_nat h0 qZ)) (fromDomain_ (as_nat h0 qZ)) prime256;
-     lemma_mod_mul_distr_l (fromDomain_ (as_nat h0 pZ) * fromDomain_ (as_nat h0 pZ)) (fromDomain_ (as_nat h0 pZ)) prime256;
-     lemma_mod_mul_distr_l (fromDomain_ (as_nat h0 qZ) * fromDomain_ (as_nat h0 qZ)) (fromDomain_ (as_nat h0 pX)) prime256;   
+  let prime = getPrime c in 
+
+     lemma_mod_mul_distr_l (fromDomain_ #c (as_nat c h0 qZ) * fromDomain_ #c (as_nat c h0 qZ)) (fromDomain_ #c (as_nat c h0 qZ)) prime;
+     lemma_mod_mul_distr_l (fromDomain_ #c (as_nat c h0 pZ) * fromDomain_ #c (as_nat c h0 pZ)) (fromDomain_ #c (as_nat c h0 pZ)) prime;
+     lemma_mod_mul_distr_l (fromDomain_ #c (as_nat c h0 qZ) * fromDomain_ #c (as_nat c h0 qZ)) (fromDomain_ #c (as_nat c h0 pX)) prime;   
      
-     lemma_mod_mul_distr_l (fromDomain_ (as_nat h0 pZ) * fromDomain_ (as_nat h0 pZ)) (fromDomain_ (as_nat h0 qX)) prime256;
-     lemma_mod_mul_distr_l (fromDomain_ (as_nat h0 qZ) * fromDomain_ (as_nat h0 qZ) * fromDomain_ (as_nat h0 qZ)) (fromDomain_ (as_nat h0 pY)) prime256;
-     lemma_mod_mul_distr_l (fromDomain_ (as_nat h0 pZ) * fromDomain_ (as_nat h0 pZ) * fromDomain_ (as_nat h0 pZ)) (fromDomain_ (as_nat h0 qY)) prime256 *)
-
+     lemma_mod_mul_distr_l (fromDomain_ #c (as_nat c h0 pZ) * fromDomain_ #c (as_nat c h0 pZ)) (fromDomain_ #c (as_nat c h0 qX)) prime;
+     lemma_mod_mul_distr_l (fromDomain_ #c (as_nat c h0 qZ) * fromDomain_ #c (as_nat c h0 qZ) * fromDomain_ #c (as_nat c h0 qZ)) (fromDomain_ #c (as_nat c h0 pY)) prime;
+     lemma_mod_mul_distr_l (fromDomain_ #c (as_nat c h0 pZ) * fromDomain_ #c (as_nat c h0 pZ) * fromDomain_ #c (as_nat c h0 pZ)) (fromDomain_ #c (as_nat c h0 qY)) prime
 
 
 inline_for_extraction noextract 
-val compute_common_params_point_add: #c: curve -> h: felem c -> r: felem c -> uh: felem c -> hCube: felem c -> 
-  u1: felem c -> u2: felem c -> s1: felem c -> s2: felem c -> tempBuffer: lbuffer uint64 (size 16) -> 
+val compute_common_params_point_add: #c: curve -> h: felem c -> r: felem c -> uh: felem c -> 
+  hCube: felem c -> u1: felem c -> u2: felem c -> s1: felem c -> s2: felem c -> 
+  tempBuffer: lbuffer uint64 (size 4 *! getCoordinateLenU64 c) -> 
   Stack unit 
-    (requires fun h0 -> live h0 h /\ live h0 r /\ live h0 uh /\ live h0 hCube /\ live h0 u1 /\ live h0 u2 /\ live h0 s1 /\ live h0 s2 /\ live h0 tempBuffer /\  
+    (requires fun h0 -> 
+      let prime = getPrime c in 
+      live h0 h /\ live h0 r /\ live h0 uh /\ live h0 hCube /\ live h0 u1 /\ 
+      live h0 u2 /\ live h0 s1 /\ live h0 s2 /\ live h0 tempBuffer /\  
       LowStar.Monotonic.Buffer.all_disjoint [loc u1; loc u2; loc s1; loc s2; loc h; loc r; loc uh; loc hCube; loc tempBuffer] /\ 
-      (
-	let prime = getPrime c in 
-	as_nat c h0 u1 < prime /\ 
-	as_nat c h0 u2 < prime /\ 
-	as_nat c h0 s1 < prime /\ 
-	as_nat c h0 s2 < prime)
-)
-    (ensures fun h0 _ h1 ->  
-      modifies (loc h |+| loc r |+| loc uh |+| loc hCube |+| loc tempBuffer) h0 h1 /\ 
-
-    (
+      as_nat c h0 u1 < prime /\ 
+      as_nat c h0 u2 < prime /\ 
+      as_nat c h0 s1 < prime /\ 
+      as_nat c h0 s2 < prime)
+    (ensures fun h0 _ h1 -> 
+      modifies (loc h |+| loc r |+| loc uh |+| loc hCube |+| loc tempBuffer) h0 h1 /\ (
       let prime = getPrime c in 
       as_nat c h1 h < prime /\ 
       as_nat c h1 r < prime /\ 
       as_nat c h1 uh < prime /\ 
-      as_nat c h1 hCube < prime /\
-      (
-	let u1D = fromDomain_ #c (as_nat c h0 u1) in 
-	let u2D = fromDomain_ #c (as_nat c h0 u2) in 
-	let s1D = fromDomain_ #c (as_nat c h0 s1) in 
-	let s2D = fromDomain_ #c (as_nat c h0 s2) in 
+      as_nat c h1 hCube < prime /\ (
+      
+      let u1D = fromDomain_ #c (as_nat c h0 u1) in 
+      let u2D = fromDomain_ #c (as_nat c h0 u2) in 
+      let s1D = fromDomain_ #c (as_nat c h0 s1) in 
+      let s2D = fromDomain_ #c (as_nat c h0 s2) in 
 	
-	let hD = fromDomain_ #c (as_nat c h1 h) in 
-
-	as_nat c h1 h == toDomain_ #c ((u2D - u1D) % prime256) /\
-	as_nat c h1 r == toDomain_ #c ((s2D - s1D) % prime256) /\
-	as_nat c h1 uh == toDomain_ #c (hD * hD * u1D % prime256) /\
-	as_nat c h1 hCube == toDomain_ #c (hD * hD * hD % prime256)
-	)
+      let hD = fromDomain_ #c (as_nat c h1 h) in 
+      
+      as_nat c h1 h == toDomain_ #c ((u2D - u1D) % prime) /\
+      as_nat c h1 r == toDomain_ #c ((s2D - s1D) % prime) /\
+      as_nat c h1 uh == toDomain_ #c (hD * hD * u1D % prime) /\
+      as_nat c h1 hCube == toDomain_ #c (hD * hD * hD % prime)))
   )
-)
 
 
-let compute_common_params_point_add h r uh hCube u1 u2 s1 s2 tempBuffer =  
+let compute_common_params_point_add #c h r uh hCube u1 u2 s1 s2 tempBuffer =  
     let h0 = ST.get() in 
-  let temp = sub tempBuffer (size 0) (size 4) in 
+  let len = getCoordinateLenU64 c in
+  let temp = sub tempBuffer (size 0) len in 
+  
   felem_sub u2 u1 h; 
-    let h1 = ST.get() in 
+  let h1 = ST.get() in
   felem_sub s2 s1 r; 
-    let h2 = ST.get() in   
+  let h2 = ST.get() in   
   montgomery_square_buffer h temp;
-    let h3 = ST.get() in   
+  let h3 = ST.get() in   
   montgomery_multiplication_buffer temp u1 uh;
-  montgomery_multiplication_buffer temp h hCube; () (*
+  montgomery_multiplication_buffer temp h hCube;
 
-    lemma_mod_mul_distr_l (fromDomain_ (as_nat c h2 h) * fromDomain_ (as_nat h2 h)) (fromDomain_ (as_nat h3 u1)) prime256;
-    lemma_mod_mul_distr_l (fromDomain_ (as_nat h2 h) * fromDomain_ (as_nat h2 h)) (fromDomain_ (as_nat h1 h)) prime256 *)
+  let prime = getPrime c in 
+  lemma_mod_mul_distr_l (fromDomain_ #c (as_nat c h2 h) * fromDomain_ #c (as_nat c h2 h)) (fromDomain_ #c (as_nat c h3 u1)) prime;
+  lemma_mod_mul_distr_l (fromDomain_ #c (as_nat c h2 h) * fromDomain_ #c (as_nat c h2 h)) (fromDomain_ #c (as_nat c h1 h)) prime
 
 
 inline_for_extraction noextract 
-val computeX3_point_add: #c : curve -> x3: felem c -> hCube: felem c -> uh: felem c -> r: felem c -> tempBuffer: lbuffer uint64 (size 16)->  Stack unit 
-  (requires fun h0 -> live h0 x3 /\ live h0 hCube /\ live h0 uh /\ live h0 r /\ live h0 tempBuffer /\
+val computeX3_point_add: #c : curve -> x3: felem c -> hCube: felem c -> uh: felem c -> 
+  r: felem c -> tempBuffer: lbuffer uint64 (size 4 *! getCoordinateLenU64 c) ->  
+  Stack unit 
+  (requires fun h0 -> 
+    let prime = getPrime c in  
+    live h0 x3 /\ live h0 hCube /\ live h0 uh /\ live h0 r /\ live h0 tempBuffer /\
     LowStar.Monotonic.Buffer.all_disjoint [loc x3; loc hCube; loc uh; loc r; loc tempBuffer] /\
-    (
-      let prime = getPrime c in 
-      as_nat c h0 hCube < prime /\as_nat c h0 uh < prime /\ as_nat c h0 r < prime)
-      
-  )
-  (ensures fun h0 _ h1 -> modifies (loc x3 |+| loc tempBuffer) h0 h1 /\ as_nat c h1 x3 < getPrime c /\ 
+    as_nat c h0 hCube < prime /\as_nat c h0 uh < prime /\ as_nat c h0 r < prime)
+  (ensures fun h0 _ h1 -> 
+    let prime = getPrime c in 
+    modifies (loc x3 |+| loc tempBuffer) h0 h1 /\ as_nat c h1 x3 < prime /\ 
     (
       let hCubeD = fromDomain_ #c (as_nat c h0 hCube) in 
       let uhD = fromDomain_ #c (as_nat c h0 uh) in 
       let rD = fromDomain_ #c (as_nat c h0 r) in 
-      as_nat c h1 x3 == toDomain_ #c ((rD * rD - hCubeD - 2 * uhD) % prime256)
+      as_nat c h1 x3 == toDomain_ #c ((rD * rD - hCubeD - 2 * uhD) % prime)
     )  
   )
 
 let computeX3_point_add #c x3 hCube uh r tempBuffer = 
-    let h0 = ST.get() in 
-  let rSquare = sub tempBuffer (size 0) (size 4) in 
-  let rH = sub tempBuffer (size 4) (size 4) in 
-  let twoUh = sub tempBuffer (size 8) (size 4) in 
+  let h0 = ST.get() in
+  
+  let len = getCoordinateLenU64 c in 
+  
+  let rSquare = sub tempBuffer (size 0) len in 
+  let rH = sub tempBuffer len len in 
+  let twoUh = sub tempBuffer (size 2 *! len) len in 
   montgomery_square_buffer r rSquare; 
     let h1 = ST.get() in 
   felem_sub rSquare hCube rH;
     let h2 = ST.get() in 
   multByTwo uh twoUh;
-    let h3 = ST.get() in 
-  felem_sub rH twoUh x3;  ()
-  (*
-    lemma_mod_add_distr (-fromDomain_  (as_nat c h1 hCube)) (fromDomain_ (as_nat c h0 r) * fromDomain_ (as_nat h0 r)) prime256;
-    lemma_mod_add_distr (-fromDomain_ (as_nat h3 twoUh)) (fromDomain_ (as_nat h0 r) * fromDomain_ (as_nat h0 r) - fromDomain_ (as_nat h1 hCube)) prime256;
-    lemma_mod_sub_distr (fromDomain_ (as_nat h0 r) * fromDomain_ (as_nat h0 r) - fromDomain_ (as_nat h1 hCube)) (2 * fromDomain_ (as_nat h2 uh)) prime256 *)
+    let h3 = ST.get() in
+  felem_sub rH twoUh x3; 
+
+  let prime = getPrime c in 
+  lemma_mod_add_distr (- fromDomain_ #c (as_nat c h1 hCube)) (fromDomain_ #c (as_nat c h0 r) * fromDomain_ #c (as_nat c h0 r)) prime;
+  lemma_mod_add_distr (- fromDomain_ #c (as_nat c h3 twoUh)) (fromDomain_ #c (as_nat c h0 r) * fromDomain_ #c (as_nat c h0 r) - fromDomain_ #c (as_nat c h1 hCube)) prime;
+  lemma_mod_sub_distr (fromDomain_ #c (as_nat c h0 r) * fromDomain_ #c (as_nat c h0 r) - fromDomain_ #c (as_nat c h1 hCube)) (2 * fromDomain_ #c (as_nat c h2 uh)) prime
 
 
 inline_for_extraction noextract 
 val computeY3_point_add: #c: curve -> y3: felem c -> s1: felem c -> 
-  hCube: felem c -> uh: felem c -> x3_out: felem c -> r: felem c -> tempBuffer: lbuffer uint64 (size 16) -> 
+  hCube: felem c -> uh: felem c -> x3_out: felem c -> r: felem c -> 
+  tempBuffer: lbuffer uint64 (size 4 *! getCoordinateLenU64 c) -> 
   Stack unit 
-    (requires fun h -> live h y3 /\ live h s1 /\ live h hCube /\ live h uh /\ live h x3_out /\ live h r /\ live h tempBuffer /\
+    (requires fun h -> 
+      let prime = getPrime c in 
+      live h y3 /\ live h s1 /\ live h hCube /\ live h uh /\ live h x3_out /\ 
+      live h r /\ live h tempBuffer /\ 
       LowStar.Monotonic.Buffer.all_disjoint [loc y3; loc s1; loc hCube; loc uh; loc x3_out; loc r; loc tempBuffer] /\
-	(let prime  = getPrime c in 
-	  as_nat c h s1 < prime /\ 
-	  as_nat c h hCube < prime /\
-	  as_nat c h uh < prime /\ 
-	  as_nat c h x3_out <prime /\ 
-	  as_nat c h r < prime
-)
-)
+      as_nat c h s1 < prime /\ 
+      as_nat c h hCube < prime /\
+      as_nat c h uh < prime /\ 
+      as_nat c h x3_out < prime /\ 
+      as_nat c h r < prime)
     (ensures fun h0 _ h1 -> 
-      modifies (loc y3 |+| loc tempBuffer) h0 h1 /\ as_nat c h1 y3 < getPrime c /\ 
+      let prime = getPrime c in 
+      modifies (loc y3 |+| loc tempBuffer) h0 h1 /\ as_nat c h1 y3 < prime /\ 
       (
 	let s1D = fromDomain_ #c (as_nat c h0 s1) in 
 	let hCubeD = fromDomain_ #c (as_nat c h0 hCube) in 
 	let uhD = fromDomain_ #c (as_nat c h0 uh) in 
 	let x3D = fromDomain_ #c (as_nat c h0 x3_out) in 
 	let rD = fromDomain_ #c (as_nat c h0 r) in 
-	as_nat c h1 y3 = toDomain_ #c (((uhD - x3D) * rD - s1D * hCubeD) % prime256)
-    )
-)
+	as_nat c h1 y3 = toDomain_ #c (((uhD - x3D) * rD - s1D * hCubeD) % prime))
+      )
 
     
-let computeY3_point_add y3 s1 hCube uh x3 r tempBuffer = 
-    let h0 = ST.get() in
-  let s1hCube = sub tempBuffer (size 0) (size 4) in 
-  let u1hx3 = sub tempBuffer (size 4) (size 4) in 
-  let ru1hx3 = sub tempBuffer (size 8) (size 4) in 
+let computeY3_point_add #c y3 s1 hCube uh x3 r tempBuffer = 
+  let h0 = ST.get() in
+  
+  let len = getCoordinateLenU64 c in 
+  let s1hCube = sub tempBuffer (size 0) len in 
+  let u1hx3 = sub tempBuffer len len in 
+  let ru1hx3 = sub tempBuffer (size 2 *! len) len in 
 
   montgomery_multiplication_buffer s1 hCube s1hCube;
   felem_sub uh x3 u1hx3;
   montgomery_multiplication_buffer u1hx3 r ru1hx3;
   
-    let h3 = ST.get() in () (*
-    lemma_mod_mul_distr_l (fromDomain_ (as_nat c h0 uh) - fromDomain_ (as_nat c h0 x3)) (fromDomain_ (as_nat h0 r)) prime256;
-  p256_sub ru1hx3 s1hCube y3;
-    lemma_mod_add_distr (-(fromDomain_ (as_nat h3 s1hCube)))  ((fromDomain_ (as_nat h0 uh) - fromDomain_ (as_nat h0 x3)) * fromDomain_ (as_nat h0 r))  prime256;
-    lemma_mod_sub_distr ((fromDomain_ (as_nat h0 uh) - fromDomain_ (as_nat h0 x3)) * fromDomain_ (as_nat h0 r)) (fromDomain_ (as_nat h0 s1) * fromDomain_ (as_nat h0 hCube)) prime256 *)
-
+  let h3 = ST.get() in 
+  let prime = getPrime c in
+    lemma_mod_mul_distr_l (fromDomain_ #c (as_nat c h0 uh) - fromDomain_ #c (as_nat c h0 x3)) (fromDomain_ #c (as_nat c h0 r)) prime;
+    felem_sub #c ru1hx3 s1hCube y3;
+    lemma_mod_add_distr (- (fromDomain_ #c (as_nat c h3 s1hCube)))  ((fromDomain_ #c (as_nat c h0 uh) - fromDomain_ #c (as_nat c h0 x3)) * fromDomain_ #c (as_nat c h0 r)) prime;
+    lemma_mod_sub_distr ((fromDomain_ #c (as_nat c h0 uh) - fromDomain_ #c (as_nat c h0 x3)) * fromDomain_ #c (as_nat c h0 r)) (fromDomain_ #c (as_nat c h0 s1) * fromDomain_ #c (as_nat c h0 hCube)) prime
 
 
 inline_for_extraction noextract 
-val computeZ3_point_add: #c: curve ->  z3: felem  c ->  z1: felem c -> z2: felem c -> h: felem c -> tempBuffer: lbuffer uint64 (size 16) -> 
-  Stack unit (requires fun h0 -> live h0 z3 /\ live h0 z1 /\ live h0 z2 /\ live h0 h /\ live h0 tempBuffer /\ live h0 z3 /\
-  LowStar.Monotonic.Buffer.all_disjoint [loc z1; loc z2; loc h; loc tempBuffer; loc z3] /\
-    (
-      let prime = getPrime c in 
-      as_nat c h0 z1 < prime /\ as_nat c h0 z2 < prime /\ as_nat  c h0 h < prime))
-  (ensures fun h0 _ h1 -> modifies (loc z3 |+| loc tempBuffer) h0 h1 /\ as_nat  c h1 z3 < getPrime c /\ 
+val computeZ3_point_add: #c: curve -> z3: felem  c ->  z1: felem c -> z2: felem c ->
+  h: felem c -> tempBuffer: lbuffer uint64 (size 4 *! getCoordinateLenU64 c) -> 
+  Stack unit (requires fun h0 -> 
+    let prime = getPrime c in 
+    live h0 z3 /\ live h0 z1 /\ live h0 z2 /\ live h0 h /\ 
+    live h0 tempBuffer /\ live h0 z3 /\
+    LowStar.Monotonic.Buffer.all_disjoint [loc z1; loc z2; loc h; loc tempBuffer; loc z3] /\
+    as_nat c h0 z1 < prime /\ as_nat c h0 z2 < prime /\ as_nat  c h0 h < prime)
+  (ensures fun h0 _ h1 ->
+    let prime = getPrime c in 
+    modifies (loc z3 |+| loc tempBuffer) h0 h1 /\ 
+    as_nat  c h1 z3 < getPrime c /\ 
     (
       let z1D = fromDomain_ #c (as_nat c h0 z1) in 
       let z2D = fromDomain_ #c (as_nat c h0 z2) in 
       let hD = fromDomain_ #c (as_nat c h0 h) in 
-      as_nat c h1 z3 == toDomain_ #c (z1D * z2D * hD % prime256)
+      as_nat c h1 z3 == toDomain_ #c (z1D * z2D * hD % prime)
     )  
   )  
 
+
 let computeZ3_point_add #c z3 z1 z2 h tempBuffer = 
     let h0 = ST.get() in 
-  let z1z2 = sub tempBuffer (size 0) (size 4) in
+  let z1z2 = sub tempBuffer (size 0) (getCoordinateLenU64 c) in
   montgomery_multiplication_buffer z1 z2 z1z2;
   montgomery_multiplication_buffer z1z2 h z3;
-    lemma_mod_mul_distr_l (fromDomain_ #c (as_nat c h0 z1) * fromDomain_ #c (as_nat c h0 z2)) (fromDomain_ #c (as_nat c h0 h)) prime256
+    lemma_mod_mul_distr_l (fromDomain_ #c (as_nat c h0 z1) * fromDomain_ #c (as_nat c h0 z2)) (fromDomain_ #c (as_nat c h0 h)) (getPrime c)
+
+val felem_eval: #c: curve -> h: mem -> b: lbuffer uint64 (getCoordinateLenU64 c) -> Type0
+
+let felem_eval #c h b = as_nat c h b < getPrime c
+
+#push-options "--z3rlimit 500" 
 
 
 inline_for_extraction noextract 
-val point_add_if_second_branch_impl: #c: curve -> result: point c -> p: point c -> q: point c -> u1: felem c -> u2: felem c -> s1: felem c -> 
-  s2: felem c -> r: felem c -> h: felem c -> uh: felem c -> hCube: felem c -> tempBuffer28 : lbuffer uint64 (size 28) -> 
+val point_add_if_second_branch_impl: #c: curve -> result: point c -> p: point c -> 
+  q: point c -> u1: felem c -> u2: felem c -> s1: felem c -> 
+  s2: felem c -> r: felem c -> h: felem c -> uh: felem c -> hCube: felem c -> 
+  tempBuffer28 : lbuffer uint64 (size 7 *! getCoordinateLenU64 c) -> 
   Stack unit 
-    (requires fun h0 -> live h0 result /\ live h0 p /\ live h0 q /\ live h0 u1 /\ live h0 u2 /\ live h0 s1 /\ live h0 s2 /\ live h0 r /\ live h0 h /\ live h0 uh /\ live h0 hCube /\ live h0 tempBuffer28 /\
-    (
+    (requires fun h0 -> 
       let prime = getPrime c in 
-    as_nat c h0 u1 < prime  /\ as_nat c h0 u2 < prime  /\ as_nat c h0 s1 < prime /\ as_nat c h0 s2 < prime /\ as_nat c h0 r < prime /\
-    as_nat c h0 h < prime /\ as_nat c h0 uh < prime /\ as_nat c h0 hCube < prime /\
-    
-    eq_or_disjoint p result /\
-    LowStar.Monotonic.Buffer.all_disjoint [loc p; loc q; loc u1; loc u2; loc s1; loc s2; loc r; loc h; loc uh; loc hCube; loc tempBuffer28] /\ 
-    disjoint result tempBuffer28 /\
-    
-    as_nat c h0 (gsub p (size 8) (size 4)) < prime /\ 
-    as_nat c h0 (gsub p (size 0) (size 4)) < prime /\ 
-    as_nat c h0 (gsub p (size 4) (size 4)) < prime /\
-    as_nat c h0 (gsub q (size 8) (size 4)) < prime /\ 
-    as_nat c h0 (gsub q (size 0) (size 4)) < prime /\  
-    as_nat c h0 (gsub q (size 4) (size 4)) < prime /\
-    
-    (
-      let pX, pY, pZ = as_nat c h0 (gsub p (size 0) (size 4)), as_nat c h0 (gsub p (size 4) (size 4)), as_nat c h0 (gsub p (size 8) (size 4)) in 
-      let qX, qY, qZ = as_nat c h0 (gsub q (size 0) (size 4)), as_nat c h0 (gsub q (size 4) (size 4)), as_nat c h0 (gsub q (size 8) (size 4)) in 
-      let pxD, pyD, pzD = fromDomain_ #c pX, fromDomain_ #c pY, fromDomain_ #c pZ in 
-      let qxD, qyD, qzD = fromDomain_ #c qX, fromDomain_ #c qY, fromDomain_ #c qZ in 
-
-      let u1D = fromDomain_ #c (as_nat c h0 u1) in 
-      let u2D = fromDomain_ #c (as_nat c h0 u2) in 
-      let s1D = fromDomain_ #c (as_nat c h0 s1) in 
-      let s2D = fromDomain_ #c (as_nat c h0 s2) in 
-
-      let hD = fromDomain_ #c (as_nat c h0 h) in 
+      let len = getCoordinateLenU64 c in
+      let len2 : size_t = size 2 *! len in 
       
-      as_nat c h0 u1 == toDomain_ #c (qzD * qzD * pxD % prime256) /\
-      as_nat c h0 u2 == toDomain_ #c (pzD * pzD * qxD % prime256) /\
-      as_nat c h0 s1 == toDomain_ #c (qzD * qzD * qzD * pyD % prime256) /\
-      as_nat c h0 s2 == toDomain_ #c (pzD * pzD * pzD * qyD % prime256) /\
+      live h0 result /\ live h0 p /\ live h0 q /\ live h0 u1 /\ live h0 u2 /\ live h0 s1 /\ 
+      live h0 s2 /\ live h0 r /\ live h0 h /\ live h0 uh /\ live h0 hCube /\ live h0 tempBuffer28 /\
+  
+      felem_eval #c h0 u1 /\ felem_eval #c h0 u2 /\ felem_eval #c h0 s1 /\ felem_eval #c h0 s2 /\
+      felem_eval #c h0 h /\ felem_eval #c h0 uh /\ felem_eval #c h0 r /\ felem_eval #c h0 hCube /\
+
+      eq_or_disjoint p result /\
+
+      LowStar.Monotonic.Buffer.all_disjoint [loc p; loc q; loc u1; loc u2; loc s1; loc s2; loc r; loc h; loc uh; loc hCube; loc tempBuffer28] /\ 
+      disjoint result tempBuffer28 /\
+
+      (
+	let pX = as_nat c h0 (gsub p (size 0) len) in 
+	let pY = as_nat c h0 (gsub p len len) in 
+	let pZ = as_nat c h0 (gsub p len2 len) in 
+
+	let qX = as_nat c h0 (gsub q (size 0) len) in 
+	let qY = as_nat c h0 (gsub q len len) in 
+	let qZ = as_nat c h0 (gsub q len2 len) in 
+
+	let pxD, pyD, pzD = fromDomain_ #c pX, fromDomain_ #c pY, fromDomain_ #c pZ in 
+	let qxD, qyD, qzD = fromDomain_ #c qX, fromDomain_ #c qY, fromDomain_ #c qZ in 
+
+	let u1D = fromDomain_ #c (as_nat c h0 u1) in 
+	let u2D = fromDomain_ #c (as_nat c h0 u2) in 
+	let s1D = fromDomain_ #c (as_nat c h0 s1) in 
+	let s2D = fromDomain_ #c (as_nat c h0 s2) in 
+
+	let hD = fromDomain_ #c (as_nat c h0 h) in 
       
-      as_nat c h0 h == toDomain_ #c ((u2D - u1D) % prime256) /\
-      as_nat c h0 r == toDomain_ #c ((s2D - s1D) % prime256) /\
-      as_nat c h0 uh == toDomain_ #c (hD * hD * u1D % prime256) /\
-      as_nat c h0 hCube == toDomain_ #c (hD * hD * hD % prime256) 
-  )
+	pX < prime /\ pY < prime /\ pZ < prime /\
+	qX < prime /\ qY < prime /\ qZ < prime /\
+	
+	as_nat c h0 u1 == toDomain_ #c (qzD * qzD * pxD % prime) /\
+	as_nat c h0 u2 == toDomain_ #c (pzD * pzD * qxD % prime) /\
+	as_nat c h0 s1 == toDomain_ #c (qzD * qzD * qzD * pyD % prime) /\
+	as_nat c h0 s2 == toDomain_ #c (pzD * pzD * pzD * qyD % prime) /\
+      
+	as_nat c h0 h == toDomain_ #c ((u2D - u1D) % prime) /\
+	as_nat c h0 r == toDomain_ #c ((s2D - s1D) % prime) /\
+	as_nat c h0 uh == toDomain_ #c (hD * hD * u1D % prime) /\
+	as_nat c h0 hCube == toDomain_ #c (hD * hD * hD % prime) 
+    )
 )
-)
+ 
   (ensures fun h0 _ h1 -> modifies (loc tempBuffer28 |+| loc result) h0 h1 /\
     (
       let prime = getPrime c in 
-    as_nat c h1 (gsub result (size 8) (size 4)) < prime /\ 
-    as_nat c h1 (gsub result (size 0) (size 4)) < prime /\  
-    as_nat c h1 (gsub result (size 4) (size 4)) < prime /\
-    (
-      let pX, pY, pZ = as_nat c h0 (gsub p (size 0) (size 4)), as_nat c h0 (gsub p (size 4) (size 4)), as_nat c h0 (gsub p (size 8) (size 4)) in 
-      let qX, qY, qZ = as_nat c h0 (gsub q (size 0) (size 4)), as_nat c h0 (gsub q (size 4) (size 4)), as_nat c h0 (gsub q (size 8) (size 4)) in 
-      let x3, y3, z3 = as_nat c h1 (gsub result (size 0) (size 4)), as_nat c h1 (gsub result (size 4) (size 4)), as_nat c h1 (gsub result (size 8) (size 4)) in  
+      let len = getCoordinateLenU64 c in 
+      let len2 : size_t = size 2 *! len in 
+  
+      let x3, y3, z3 = as_nat c h1 (gsub result (size 0) len), as_nat c h1 (gsub result len len), as_nat c h1 (gsub result len2 len) in  
+      
+      x3 < prime /\ y3 < prime /\ z3 < prime /\
+      (
+	let pX, pY, pZ = as_nat c h0 (gsub p (size 0) len), as_nat c h0 (gsub p len len), as_nat c h0 (gsub p len2 len) in 
+	let qX, qY, qZ = as_nat c h0 (gsub q (size 0) len), as_nat c h0 (gsub q len len), as_nat c h0 (gsub q len2 len) in 
 
-      let pxD, pyD, pzD = fromDomain_ #c pX, fromDomain_ #c pY, fromDomain_ #c pZ in 
-      let qxD, qyD, qzD = fromDomain_ #c qX, fromDomain_ #c qY, fromDomain_ #c qZ in 
-      let x3D, y3D, z3D = fromDomain_ #c x3, fromDomain_ #c y3, fromDomain_ #c z3 in 
+	let pxD, pyD, pzD = fromDomain_ #c pX, fromDomain_ #c pY, fromDomain_ #c pZ in 
+	let qxD, qyD, qzD = fromDomain_ #c qX, fromDomain_ #c qY, fromDomain_ #c qZ in 
+	let x3D, y3D, z3D = fromDomain_ #c x3, fromDomain_ #c y3, fromDomain_ #c z3 in 
 
-      let rD = fromDomain_ #c (as_nat c h0 r) in 
-      let hD = fromDomain_ #c (as_nat c h0 h) in 
-      let s1D = fromDomain_ #c (as_nat c h0 s1) in 
-      let u1D = fromDomain_ #c (as_nat c h0 u1) in 
+	let rD = fromDomain_ #c (as_nat c h0 r) in 
+	let hD = fromDomain_ #c (as_nat c h0 h) in 
+	let s1D = fromDomain_ #c (as_nat c h0 s1) in 
+	let u1D = fromDomain_ #c (as_nat c h0 u1) in 
 
-  if qzD = 0 then 
-    x3D == pxD /\ y3D == pyD /\ z3D == pzD
-   else if pzD = 0 then 
-    x3D == qxD /\  y3D == qyD /\ z3D == qzD
-   else 
-    x3 == toDomain_ #c ((rD * rD - hD * hD * hD - 2 * hD * hD * u1D) % prime256) /\ 
-    y3 == toDomain_ #c (((hD * hD * u1D - fromDomain_  #c x3) * rD - s1D * hD * hD * hD) % prime256) /\
-    z3 == toDomain_ #c (pzD * qzD * hD % prime256) 
+	if qzD = 0 then 
+	  x3D == pxD /\ y3D == pyD /\ z3D == pzD
+	else if pzD = 0 then 
+	  x3D == qxD /\  y3D == qyD /\ z3D == qzD
+	else 
+	  x3 == toDomain_ #c ((rD * rD - hD * hD * hD - 2 * hD * hD * u1D) % prime) /\ 
+	  y3 == toDomain_ #c (((hD * hD * u1D - fromDomain_  #c x3) * rD - s1D * hD * hD * hD) % prime) /\
+	  z3 == toDomain_ #c (pzD * qzD * hD % prime) 
+  )
   )
 )
-)
+
 
 let point_add_if_second_branch_impl #c result p q u1 u2 s1 s2 r h uh hCube tempBuffer28 = 
-    let h0 = ST.get() in 
-  let pZ = sub p (size 8) (size 4) in 
-  let qZ = sub q (size 8) (size 4) in 
-
-  let tempBuffer16 = sub tempBuffer28 (size 0) (size 16) in 
+  let h0 = ST.get() in
+  let len = getCoordinateLenU64 c in 
   
-  let x3_out = Lib.Buffer.sub tempBuffer28 (size 16) (size 4) in 
-  let y3_out = Lib.Buffer.sub tempBuffer28 (size 20) (size 4) in 
-  let z3_out = Lib.Buffer.sub tempBuffer28 (size 24) (size 4) in 
+  let pZ = sub p (size 2 *! len) len in 
+  let qZ = sub q (size 2 *! len) len in 
 
+  let tempBuffer16 = sub tempBuffer28 (size 0) (size 4 *! len) in admit();
+  
+  let x3_out = Lib.Buffer.sub tempBuffer28 (size 4 *! len) len in 
+  let y3_out = Lib.Buffer.sub tempBuffer28 (size 5 *! len) len in 
+  let z3_out = Lib.Buffer.sub tempBuffer28 (size 6 *! len) len in admit();
+  
   computeX3_point_add x3_out hCube uh r tempBuffer16; 
     let h1 = ST.get() in 
   computeY3_point_add y3_out s1 hCube uh x3_out r tempBuffer16; 
   computeZ3_point_add z3_out pZ qZ h tempBuffer16;
+  
   copy_point_conditional x3_out y3_out z3_out q p;
-
   copy_point_conditional x3_out y3_out z3_out p q;
-  concat3 (size 4) x3_out (size 4) y3_out (size 4) z3_out result; 
 
-    let hEnd = ST.get() in 
+  concat3 len x3_out len y3_out len z3_out result; 
+
+  let hEnd = ST.get() in 
+
+  let prime = getPrime c in 
 
   let rD = fromDomain_ #c (as_nat c h0 r) in 
   let hD = fromDomain_ #c (as_nat c h0 h) in
@@ -584,60 +641,71 @@ let point_add_if_second_branch_impl #c result p q u1 u2 s1 s2 r h uh hCube tempB
 
   let s1D = fromDomain_ #c (as_nat c h0 s1) in 
   let x3D = fromDomain_ #c (as_nat c h1 x3_out) in 
-(*
-  lemma_point_add_0 (rD * rD) (hD * hD * hD) (hD * hD * u1D);
-  lemma_mod_sub_distr (rD * rD - 2 * uhD) (hD * hD * hD) prime256;
+
+  lemma_point_add_0 #c (rD * rD) (hD * hD * hD) (hD * hD * u1D);
+  lemma_mod_sub_distr (rD * rD - 2 * uhD) (hD * hD * hD) prime;
   assert_by_tactic (2 * (hD * hD * u1D) == 2 * hD * hD * u1D) canon;
 
-  lemma_point_add_1 (hD * hD * u1D) x3D rD s1D (hD * hD * hD);
+  lemma_point_add_1 #c (hD * hD * u1D) x3D rD s1D (hD * hD * hD);
   assert_by_tactic (s1D * (hD * hD * hD) == s1D * hD * hD * hD) canon;
 
-  assert_norm (modp_inv2 #P256 (pow2 256) > 0);
-  assert_norm (modp_inv2 #P256 (pow2 256) % prime <> 0); 
+  assert_norm (modp_inv2 #P256 (getPower2 P256) > 0);
+  assert_norm (modp_inv2 #P384 (getPower2 P384) > 0);
+  
+  assert_norm (modp_inv2 #P256 (getPower2 P256) % prime <> 0); 
+  assert_norm (modp_inv2 #P384 (getPower2 P384) % prime <> 0); 
 
-  lemma_multiplication_not_mod_prime (as_nat h0 pZ);
-  lemma_multiplication_not_mod_prime (as_nat h0 qZ);
-  lemmaFromDomain (as_nat h0 pZ);
-  lemmaFromDomain (as_nat h0 qZ) *) ()
+  lemma_multiplication_not_mod_prime (as_nat c h0 pZ);
+  lemma_multiplication_not_mod_prime (as_nat c h0 qZ);
+  lemmaFromDomain #c (as_nat c h0 pZ);
+  lemmaFromDomain #c (as_nat c h0 qZ);
+  admit()
+
+#pop-options
 
 
 let point_add #c p q result tempBuffer = 
-    let h0 = ST.get() in 
+  let h0 = ST.get() in 
+
+  let len = getCoordinateLenU64 c in 
   
-  let z1 = sub p (size 8) (size 4) in 
-  let z2 = sub q (size 8) (size 4) in 
+  let z1 = sub p (size 2 *! len) len in 
+  let z2 = sub q (size 2 *! len) len in 
 
-  let tempBuffer16 = sub tempBuffer (size 0) (size 16) in 
+  let tempBuffer16 = sub tempBuffer (size 0) (size 4 *! len) in 
    
-  let u1 = sub tempBuffer (size 16) (size 4) in 
-  let u2 = sub tempBuffer (size 20) (size 4) in 
-  let s1 = sub tempBuffer (size 24) (size 4) in 
-  let s2 = sub tempBuffer (size 28) (size 4) in 
+  let u1 = sub tempBuffer (size 4 *! len) len in 
+  let u2 = sub tempBuffer (size 5 *! len) len in 
+  let s1 = sub tempBuffer (size 6 *! len) len in 
+  let s2 = sub tempBuffer (size 7 *! len) len in 
 
-  let h = sub tempBuffer (size 32) (size 4) in 
-  let r = sub tempBuffer (size 36) (size 4) in 
-  let uh = sub tempBuffer (size 40) (size 4) in 
+  let h = sub tempBuffer (size 8 *! len) len in 
+  let r = sub tempBuffer (size 9 *! len) len in 
+  let uh = sub tempBuffer (size 10 *! len) len in 
 
-  let hCube = sub tempBuffer (size 44) (size 4) in 
+  let hCube = sub tempBuffer (size 11 *! len) len in 
 
-  let x3_out = sub tempBuffer (size 48) (size 4) in 
-  let y3_out = sub tempBuffer (size 52) (size 4) in 
-  let z3_out = sub tempBuffer (size 56) (size 4) in 
+  let x3_out = sub tempBuffer (size 12 *! len) len in 
+  let y3_out = sub tempBuffer (size 13 *! len) len in 
+  let z3_out = sub tempBuffer (size 14 *! len) len in 
 
-  let tempBuffer28 = sub tempBuffer (size 60) (size 28) in 
+  let tempBuffer28 = sub tempBuffer (size 15 *! len) (size 7 *! len) in 
   
   move_from_jacobian_coordinates u1 u2 s1 s2 p q tempBuffer16;
   compute_common_params_point_add #c h r uh hCube u1 u2 s1 s2 tempBuffer16;
   point_add_if_second_branch_impl result p q u1 u2 s1 s2 r h uh hCube tempBuffer28;
+  
     let h1 = ST.get() in 
-      let pxD = fromDomain_ #c (as_nat c h0 (gsub p (size 0) (size 4))) in 
-      let pyD = fromDomain_ #c (as_nat c h0 (gsub p (size 4) (size 4))) in 
-      let pzD = fromDomain_ #c (as_nat c h0 (gsub p (size 8) (size 4))) in 
-      let qxD = fromDomain_ #c (as_nat c h0 (gsub q (size 0) (size 4))) in 
-      let qyD = fromDomain_ #c (as_nat c h0 (gsub q (size 4) (size 4))) in 
-      let qzD = fromDomain_ #c (as_nat c h0 (gsub q (size 8) (size 4))) in 
-      let x3 = as_nat c h1 (gsub result (size 0) (size 4)) in 
-      let y3 = as_nat c h1 (gsub result (size 4) (size 4)) in 
-      let z3 = as_nat c h1 (gsub result (size 8) (size 4)) in 
+      let pxD = fromDomain_ #c (as_nat c h0 (gsub p (size 0) len)) in 
+      let pyD = fromDomain_ #c (as_nat c h0 (gsub p len len)) in 
+      let pzD = fromDomain_ #c (as_nat c h0 (gsub p (size 2 *! len) len)) in
+      
+      let qxD = fromDomain_ #c (as_nat c h0 (gsub q (size 0) len)) in 
+      let qyD = fromDomain_ #c (as_nat c h0 (gsub q len len)) in 
+      let qzD = fromDomain_ #c (as_nat c h0 (gsub q (size 2 *! len) len)) in 
+      
+      let x3 = as_nat c h1 (gsub result (size 0) len) in 
+      let y3 = as_nat c h1 (gsub result len len) in 
+      let z3 = as_nat c h1 (gsub result (size 2 *! len) len) in 
       lemma_pointAddToSpecification #c  pxD pyD pzD qxD qyD qzD x3 y3 z3 (as_nat c h1 u1) (as_nat c h1 u2) (as_nat c h1 s1) (as_nat c h1 s2) (as_nat c h1 h) (as_nat c h1 r)
 
