code/ecdsap256/Hacl.Impl.P256.PointAdd.fsti
@@ -29,28 +29,40 @@ open FStar.Math.Lemmas
 
 open FStar.Mul
 
-#reset-options "--z3rlimit 300" 
+#set-options "--z3rlimit 100"
 
 val point_add: #c: curve -> p: point c -> q: point c -> result: point c -> tempBuffer: lbuffer uint64 (size 88) -> 
-   Stack unit (requires fun h -> live h p /\ live h q /\ live h result /\ live h tempBuffer /\ 
-   eq_or_disjoint q result /\
-   disjoint p q /\ disjoint p tempBuffer /\ disjoint q tempBuffer /\ disjoint p result /\ disjoint result tempBuffer /\  
-    as_nat c h (gsub p (size 8) (size 4)) < prime256 /\ 
-    as_nat c h (gsub p (size 0) (size 4)) < prime256 /\ 
-    as_nat c h (gsub p (size 4) (size 4)) < prime256 /\
-    as_nat c h (gsub q (size 8) (size 4)) < prime256 /\ 
-    as_nat c h (gsub q (size 0) (size 4)) < prime256 /\  
-    as_nat c h (gsub q (size 4) (size 4)) < prime256 
-    ) 
+   Stack unit (requires fun h -> 
+     live h p /\ live h q /\ live h result /\ live h tempBuffer /\ 
+     eq_or_disjoint q result /\ disjoint p q /\ disjoint p tempBuffer /\ 
+     disjoint q tempBuffer /\ disjoint p result /\ disjoint result tempBuffer /\  
+    (
+      let prime = getPrime c in 
+      let len = getCoordinateLenU64 c in 
+      
+      as_nat c h (gsub p (size 0) len) < prime /\ 
+      as_nat c h (gsub p len len) < prime /\ 
+      as_nat c h (gsub p (size 2 *! len) len) < prime /\
+      
+      as_nat c h (gsub q (size 0) len) < prime /\ 
+      as_nat c h (gsub q len len) < prime /\ 
+      as_nat c h (gsub q (size 2 *! len) len) < prime
+      )
+   )
    (ensures fun h0 _ h1 -> 
      modifies (loc tempBuffer |+| loc result) h0 h1 /\ 
-     as_nat c h1 (gsub result (size 8) (size 4)) < prime256 /\ 
-     as_nat c h1 (gsub result (size 0) (size 4)) < prime256 /\ 
-     as_nat c h1 (gsub result (size 4) (size 4)) < prime256 /\
      (
-       let pX, pY, pZ = gsub p (size 0) (size 4), gsub p (size 4) (size 4), gsub p (size 8) (size 4) in 
-       let qX, qY, qZ = gsub q (size 0) (size 4), gsub q (size 4) (size 4), gsub q (size 8) (size 4) in 
-       let x3, y3, z3 = gsub result (size 0) (size 4), gsub result (size 4) (size 4), gsub result (size 8) (size 4) in 
+       let len : size_t = getCoordinateLenU64 c in 
+       let prime = getPrime c in 
+     
+       as_nat c h1 (gsub result (size 0) len) < prime /\ 
+       as_nat c h1 (gsub result len len) < prime /\ 
+       as_nat c h1 (gsub result (2ul *! len) len) < prime /\
+       
+       (
+       let pX, pY, pZ = gsub p (size 0) len, gsub p len len, gsub p (size 2 *! len) len in 
+       let qX, qY, qZ = gsub q (size 0) len, gsub q len len, gsub q (size 2 *! len) len in 
+       let x3, y3, z3 = gsub result (size 0) len, gsub result len len, gsub result (size 2 *! len) len in 
        
        let pxD, pyD, pzD = fromDomain_ #c (as_nat c h0 pX), fromDomain_ #c (as_nat c h0 pY), fromDomain_ #c (as_nat c h0 pZ) in 
        let qxD, qyD, qzD = fromDomain_ #c (as_nat c h0 qX), fromDomain_ #c (as_nat c h0 qY), fromDomain_ #c (as_nat c h0 qZ) in 
@@ -58,5 +70,6 @@ val point_add: #c: curve -> p: point c -> q: point c -> result: point c -> tempB
       
        let xN, yN, zN = _point_add #c (pxD, pyD, pzD) (qxD, qyD, qzD) in 
        x3D == xN /\ y3D == yN /\ z3D == zN
-  )
-)
+   )
+   )
+   )
